verified, needs to do refinment laws

InsertionSort.dfy
@@ -1,6 +1,7 @@
+
 method PairInsertionSort(a: array<int>)
 	requires a.Length>1
-	ensures Sorted(a,0,a.Length-1)
+	ensures Sorted1(a,0,a.Length-1)
 	ensures multiset(a[..]) == multiset(old(a[..]))
 	modifies a
 {
@@ -9,34 +10,38 @@ method PairInsertionSort(a: array<int>)
 	i:=0;
 	j:=i-1;
 	while i < a.Length-1
-		decreases (a.Length-1) - i
-		invariant Inv(a[..],i,j,A)
+		decreases a.Length - i
+		invariant InvPair(a[..],i,j,A)
 	{
 		x,y:=a[i],a[i+1];
 		if x<y {
 			x,y:=y,x;
 		}
-		j:= i-1;
+		else{
 
+		} 
+		j:= i-1;
 		while j>=0 && a[j]>x
-			invariant Inv2(a[..],j,i,x,y,A)
+			invariant Inv2Pair(a[..],j,i,x,y,A)
 			decreases j
 			{
-				Swap(a,j+2,j,A);
+				SwapPair(a,j+2,j,A);
 				j:=j-1;
 			}
 		if a[j+2]!=x{
-			Swap(a,j+2,j+1,A);
+			LemmaMidswap(a[..],j,i,x,y,A);
+			SwapPair(a,j+2,j+1,A);
 		}	
 		else{
-
+			LemmaMidNoswap(a[..],j,i,x,y,A);
 		}
-
+		
+		
 		while j>=0 && a[j] > y
-			invariant Inv3(a[..],j,i,x,y,A)
+			invariant Inv3Pair(a[..],j,i,x,y,A)
 			decreases j
 			{
-				Swap(a,j+1,j,A);
+				SwapPair(a,j+1,j,A);
 				j:=j-1;
 			}
 		
@@ -46,80 +51,111 @@ method PairInsertionSort(a: array<int>)
 	if i==a.Length-1{
 		j,y := i-1,a[i];
 		while j>=0 && a[j] >y
-			invariant Inv4(a[..],j,i,x,y,A)
+			invariant Inv4Pair(a[..],j,i,x,y,A)
 			decreases j
 		{
-			Swap(a,j+1,j,A);
+			SwapPair(a,j+1,j,A);
 			j:=j-1;
 		}
 	}
 	else {
 
-	}
-			
-		
+	}	
 
 }
 
-predicate Sorted(a: array<int>, i:nat, j:int)
-	requires j>0 
+
+predicate Inv2Pair(a: seq<int>, j: int,i:nat,x:int, y:int, A: multiset<int>)
+{
+	0<=i<=|a|-2 &&
+	-1<=j<=|a|-3 &&
+	SortedSequence1(a,0,j)&&
+	SortedSequence1(a,j+2,i+1)&&
+	(0<=j<i-1 ==> a[j+3]>=a[j]) &&
+	(j<i-1  ==> a[j+3]>x) &&
+	((x==a[j+1]&&y==a[j+2]) || (x==a[j+2]&&y==a[j+1])) && x>=y &&
+	multiset(a)==A
+}
+
+predicate Sorted1(a: array<int>, i:nat, j:int)
 	requires i<=j ==> (0<=i<a.Length && 0<=j<a.Length)
 	reads a
 {
-	 (forall k :: i <= k < j-1 ==> a[k] <= a[k+1]) || a.Length<=1
+	 (forall k :: i <= k < j-1 ==> a[k] <= a[k+1]) 
 }
-
-predicate SortedSequence(a: seq<int>, i:nat, j:int)
-	requires j>0 
-	requires i<=j ==> (0<=i<|a| && 0<=j<|a|)
+predicate InvPair(a: seq<int>, i: nat, j:int, A: multiset<int>)
 {
-	(forall k :: i <= k < j-1 ==> a[k] <= a[k+1]) || |a|<=1
+	0<=i<=|a| &&
+	(-1<=j<=|a|-3) &&
+	SortedSequence1(a,0,i-1) &&
+	multiset(a)==A
 }
-predicate Inv(a: seq<int>, i: nat, j:int, A: multiset<int>)
+
+predicate SortedSequence1(a: seq<int>, i:nat, h:int)
+	requires i<=h ==> (0<=i <|a| && 0<=h<|a|)
 {
-	0<=i<|a|-2 &&
-	-1<=j<|a|-3 &&
-	SortedSequence(a,0,i+1) &&
-	multiset(a) == A
+	(forall k :: i <=  k <= h-1 ==> a[k] <= a[k+1])
 }
-predicate Inv2(a: seq<int>, j: int,i:nat,x:int, y:int, A: multiset<int>)
+
+lemma LemmaMidswap(a: seq<int>,j:int,i:nat,x:int,y:int, A: multiset<int>)
+	requires Inv2Pair(a,j,i,x,y,A)
+	requires j<0 || a[j]<=x
+	requires a[j+2]!=x
+	ensures Inv3Pair(a[j+1:=a[j+2]][j+2:=a[j+1]],j,i,x,y,A)
 {
-	0<=j<=|a|-3&&
-	SortedSequence(a,0,j-1)&&
-	SortedSequence(a,j+2,i+1)&& 
-	(j>0 ==> a[j+2]>=a[j-1]) &&
-	a[j+2]>x &&
-	multiset(a) == A&&
-	((a[j] == x && a[j+1] == y) || (a[j]==y && a[j+1] == x))
 }
 
-predicate Inv3(a: seq<int>, j: int,i:nat,x:int, y:int, A: multiset<int>)
+lemma LemmaMidNoswap(a: seq<int>,j:int,i:nat,x:int,y:int, A: multiset<int>)
+	requires Inv2Pair(a,j,i,x,y,A)
+	requires j<0 || a[j]<=x
+	requires a[j+2]==x
+	ensures Inv3Pair(a,j,i,x,y,A)
 {
-	0<=j<=|a|-3&&
-	SortedSequence(a,0,j-1)&&
-	SortedSequence(a,j+1,i+1)&& 
-	(j>0 ==> a[j+1]>=a[j-1]) &&
-	a[j+1]>y &&
-	multiset(a) == A&&
-	a[j] == y 
 }
 
-predicate Inv4(a: seq<int>, j: int,i:nat,x:int, y:int, A: multiset<int>)
+lemma firstLoop(a: seq<int>,j:int,i:nat,x:int,y:int, A: multiset<int>)
+	requires Inv2Pair(a,j,i,x,y,A) && j>=0 && a[j] > x
+	ensures Inv2Pair(a[j:=a[j+2]][j+2:=a[j]],j-1,i,x,y,A)
+{}
+lemma secondLoop(a: seq<int>,j:int,i:nat,x:int,y:int, A: multiset<int>)
+	requires Inv3Pair(a[..],j,i,x,y,A) && j>=0 && a[j] > y
+	ensures Inv3Pair(a[j:=a[j+1]][j+1:=a[j]],j-1,i,x,y,A)
+{}
+
+lemma fourthLoop(a: seq<int>,j:int,i:nat,x:int,y:int, A: multiset<int>)
+	requires Inv4Pair(a[..],j,i,x,y,A) && j>=0 && a[j] > y
+	ensures Inv4Pair(a[j:=a[j+1]][j+1:=a[j]],j-1,i,x,y,A)
 {
-	0<=j<=|a|-2&&
-	SortedSequence(a,0,j-1)&&
-	SortedSequence(a,j+1,|a|-1)&& 
-	(j>0 ==> a[j+1]>=a[j-1]) &&
-	a[j+1]>y &&
-	multiset(a) == A&&
-	a[j] == y 
+}
+
+predicate Inv3Pair(a: seq<int>, j: int,i:nat,x:int, y:int, A: multiset<int>)
+{
+	0<=i<=|a|-2 &&
+	-1<=j<=|a|-3 &&
+	SortedSequence1(a,0,j)&&
+	SortedSequence1(a,j+1,i+1)&&
+	a[j+2]>=y &&
+	(j>=0 ==> a[j+2]>=a[j]) &&
+	a[j+1]==y &&
+	multiset(a)==A
+}
+
+predicate Inv4Pair(a: seq<int>, j: int,i:nat,x:int, y:int, A: multiset<int>)
+{
+	-1<=j<=|a|-2&&
+	SortedSequence1(a,0,j)&&
+	SortedSequence1(a,j+2,|a|-1)&&
+	a[j+1]==y && 
+	(j<=|a|-3 ==> a[j+2]>y) &&
+	(0<=j<=|a|-3 ==> a[j+2]>=a[j]) &&
+	multiset(a)==A
 }
 
 
 
 
 
-method {:verify true} Swap(a: array<int>, x:nat,y:nat,ghost A: multiset<int>)
+method {:verify true} SwapPair(a: array<int>, x:nat,y:nat,ghost A: multiset<int>)
 	requires multiset(a[..]) == A
 	requires 0<=x<a.Length && 0<=y<a.Length
 	requires x!=y
@@ -130,21 +166,17 @@ method {:verify true} Swap(a: array<int>, x:nat,y:nat,ghost A: multiset<int>)
 	modifies a
 {
 	// assignment
-	LemmaSwap(a[..],old(a[..]), x, y, A);
+	LemmaSwapPair(a[..],old(a[..]), x, y, A);
 	a[x], a[y] := a[y], a[x];
 }
 
-lemma LemmaSwap(a: seq<int>,oldA :seq <int>, x: nat, y: nat, A: multiset<int>)
-	requires |a|==|oldA|
-	requires forall i:: 0<=i<|a| ==> a[i]==oldA[i]
+lemma LemmaSwapPair(a: seq<int>,oldA :seq <int>, x: nat, y: nat, A: multiset<int>)
+	requires a==oldA
+	requires multiset(a[..]) == A
 	requires 0<=x<|a| && 0<=y<|a|
 	requires x!=y
+	ensures multiset(a[x:= oldA[y]][y:=oldA[x]]) == A
 	ensures a[x:= oldA[y]][y:=oldA[x]][x] == oldA[y]
 	ensures  a[x:= oldA[y]][y:=oldA[x]][y] == oldA[x]
 	ensures forall i :: 0<=i<|a| ==> ((i!=x && i!=y) ==> a[x:= oldA[y]][y:=oldA[x]][i]==oldA[i])
 {}
-
-// this helps in justifying the move from the initial guard to the efficient one,
-// with no need to change anything in the initial development:
-// the (LHS ==> RHS) helps in the loop body,
-// and (LHS <== RHS) helps upon termination of the loop
